src/Iris/Algebra/CMRA.lean
@@ -1,7 +1,7 @@
 /-
 Copyright (c) 2025 Mario Carneiro. All rights reserved.
 Released under Apache 2.0 license as described in the file LICENSE.
-Authors: Mario Carneiro, Сухарик (@suhr), Markus de Medeiros
+Authors: Mario Carneiro, Сухарик (@suhr), Markus de Medeiros, Puming Liu
 -/
 import Iris.Algebra.OFE
 
@@ -1365,6 +1365,18 @@ theorem valid_snd {x : α × β} (h : ✓ x) : ✓ x.snd := h.right
 theorem validN_fst {n} {x : α × β} (h : ✓{n} x) : ✓{n} x.fst := h.left
 theorem validN_snd {n} {x : α × β} (h : ✓{n} x) : ✓{n} x.snd := h.right
 
+theorem incN_iff {n} (a a' : α) (b b' : β) :
+    a ≼{n} a' ∧ b ≼{n} b' ↔ (a, b) ≼{n} (a', b') := by
+  constructor
+  · simp [CMRA.IncludedN]
+    rintro x hx y hy
+    exact ⟨x, ⟨y, ⟨hx, hy⟩⟩⟩
+  · simp [CMRA.IncludedN]
+    rintro x y ⟨ha, hb⟩
+    constructor
+    · exact ⟨x, Option.dist_of_some_dist_some ha⟩
+    · exact ⟨y, Option.dist_of_some_dist_some hb⟩
+
 instance [CMRA.Discrete α] [CMRA.Discrete β]: CMRA.Discrete (α × β) where
   discrete_valid := by
     rintro ⟨_, _⟩
@@ -1372,6 +1384,78 @@ instance [CMRA.Discrete α] [CMRA.Discrete β]: CMRA.Discrete (α × β) where
     exact (⟨CMRA.discrete_valid ·, CMRA.discrete_valid ·⟩)
 
 end Prod
+
+section ProdOF
+
+open COFE
+
+variable [OFE A] [OFE A'] [OFE B] [OFE B']
+
+
+instance (f : A → A') (g : B → B') [NonExpansive f] [NonExpansive g] :
+    NonExpansive (Prod.map f g) where
+  ne _ _ _ H := by
+    constructor
+    · rw [Prod.map_fst]
+      exact NonExpansive.ne H.1
+    · rw [Prod.map_snd]
+      exact NonExpansive.ne H.2
+
+omit [OFE A] [OFE B] in
+theorem Prod.map_ext {f f' : A → A'} {g g' : B → B'} (Hf : ∀ a, f a ≡ f' a)
+    (Hg : ∀ a, g a ≡ g' a) : Prod.map f g x ≡ Prod.map f' g' x :=
+  ⟨Hf x.fst, Hg x.snd⟩
+
+omit [OFE A] [OFE B] in
+theorem Prod.map_ne {f f' : A → A'} {g g' : B → B'} (Hf : ∀ a, f a ≡{n}≡ f' a)
+    (Hg : ∀ a, g a ≡{n}≡ g' a) : Prod.map f g x ≡{n}≡ Prod.map f' g' x :=
+  ⟨Hf x.fst, Hg x.snd⟩
+
+instance Prod.mapO (f : A -n> A') (g : B -n> B') : A × B -n> A' × B' where
+  f := .map f g
+  ne := inferInstance
+
+abbrev ProdOF (F1 F2 : OFunctorPre) : OFunctorPre := fun A B => (F1 A B) × (F2 A B)
+
+open OFunctor in
+instance [OFunctor F1] [OFunctor F2] : OFunctor (ProdOF F1 F2) where
+  cofe := inferInstance
+  map f g := Prod.mapO (map f g) (map f g)
+  map_ne.ne _ _ _ Hx _ _ Hy _ := ⟨map_ne.ne Hx Hy _, map_ne.ne Hx Hy _⟩
+  map_id _ := ⟨map_id _, map_id _⟩
+  map_comp _ _ _ _ _ := ⟨map_comp .., map_comp ..⟩
+
+open OFunctorContractive in
+instance [OFunctorContractive F1] [OFunctorContractive F2] : OFunctorContractive (ProdOF F1 F2) where
+  map_contractive.1 H _ :=
+    Prod.map_ne (fun _ => map_contractive.1 H _) (fun _ => map_contractive.1 H _)
+
+end ProdOF
+
+section ProdMor
+
+open CMRA
+
+variable [CMRA A] [CMRA A'] [CMRA B] [CMRA B']
+
+instance Prod.mapC (f : A -C> A') (g : B -C> B') : A × B -C> A' × B' where
+  f := Prod.map f g
+  ne := inferInstance
+  validN {n x} := fun ⟨h1, h2⟩ => ⟨Hom.validN _ h1, Hom.validN _ h2⟩
+  pcore x := by
+    simp [Option.map, Prod.map, CMRA.pcore, pcore]
+    have h2 := Hom.pcore g x.snd
+    have h1 := Hom.pcore f x.fst
+    cases _ : CMRA.pcore x.fst
+    · cases _ : CMRA.pcore (f.f x.fst) <;> simp_all
+    · cases _ : CMRA.pcore x.snd <;>
+      cases _ : CMRA.pcore (f.f x.fst) <;>
+      cases _ : CMRA.pcore (g.f x.snd) <;>
+      simp_all
+      exact ⟨Option.equiv_of_some_equiv_some h1, Option.equiv_of_some_equiv_some h2⟩
+  op x y := ⟨CMRA.Hom.op .., CMRA.Hom.op ..⟩
+
+end ProdMor
 
 section optionOF
 
